MachCSL/WpSmodeMint.lean
@@ -182,7 +182,7 @@ theorem wp_s_sd_mint [CurCtx] [KernelGeom] [KernelImage GF] (cpu : CPU) (k : KCt
         iexact Hkey
     · inext
       iintro HmConf HPC HnextPC ⟨Htrans, Hfrag, HF, Hctx, Hcell⟩
-      ihave Htok := ctxTok_intro cpu' curCtx none $$ [Hctx Hfrag]
+      ihave Htok := ctxTok_introB cpu' curCtx none false $$ [Hctx Hfrag]
       case' _ => iframe
       ihave HT := transTok_intro cpu' curTier k.root $$ [Htrans Htok]
       case' _ => iframe
@@ -268,7 +268,7 @@ theorem wp_s_sw_mint [CurCtx] [KernelGeom] [KernelImage GF] (cpu : CPU) (k : KCt
         iexact Hkey
     · inext
       iintro HmConf HPC HnextPC ⟨Htrans, Hfrag, HF, Hctx, Hcell⟩
-      ihave Htok := ctxTok_intro cpu' curCtx none $$ [Hctx Hfrag]
+      ihave Htok := ctxTok_introB cpu' curCtx none false $$ [Hctx Hfrag]
       case' _ => iframe
       ihave HT := transTok_intro cpu' curTier k.root $$ [Htrans Htok]
       case' _ => iframe
